src/ExpandWhens_radical_rewrite.v
@@ -1,0 +1,787 @@
+(* Expand Whens pass
+
+   This is part of the Hardware Verification project of ISCAS,
+   under the leadership of Prof. Zhilin Wu.
+   This file has been written mainly by David N. Jansen.
+
+   Expand Whens is part of the translation from HiFirrtl to LoFirrtl.
+   Before Expand Whens, all widths have been inferred and all types
+   lowered, so we just assume this as preconditions.
+   The main duty of the Expand Whens pass is to replace all when
+   statements with suitable multiplexers.  In this process, also
+   the “last connect” semantics is ensured.
+
+   The main function of Expand Whens is ExpandBranch_funs.  This
+   function extracts the component definition statements from a
+   statement sequence, puts them in a linear statement sequence
+   (i.e. removes all when statements here), and it also extracts
+   a connection map that describes how every component is connected.
+   This connection map is then written out as a sequence of
+   connect statements (and possibly “is invalid” statements).
+
+   A compiler (part) is correct if: every semantics of a translated
+   design is also a semantics of the original design.  In
+   particular, an incorrect design -- a program without semantics --
+   is not translated to a correct design.  Therefore, ExpandBranch_funs
+   also has to check for some errors, namely those that could
+   disappear by expanding when statements.  These are:
+   - scoping errors: a component is defined within a branch of a
+     when statement but accesses outside.
+   - connection errors: an erroneous connection (type or flow
+     direction) is made but later overwritten.
+   - condition type errors: a when statement condition contains
+     an error but the condition actually never needs to be evaluated
+     in the translated design.
+   Note that strictly speaking, some errors can be left alone;
+   for example, if multiple components have the same name in a
+   single module, scopes do not matter, so the design will be
+   erroneous before and after Expand Whens.
+
+   Internally speaking, because all types have been lowered before,
+   the tmap (which contained the type of every component) is not
+   needed.  Expand Whens will only use the vertex set of the module
+   graph vm to decide what type and flow direction an expression has.
+
+   A remark on style: many definitions are mutually recursive because
+   statements and statement sequences are mutually recursive.  We
+   prefer to place the statement sequence function before the
+   single-statement function.
+   *)
+
+From Coq Require Import BinNat ZArith.
+From mathcomp Require Import ssreflect ssrbool eqtype seq fintype ssrnat div ssrfun.
+From simplssrlib Require Import SsrOrder Var FMaps.
+From firrtl Require Import Firrtl Env HiEnv HiFirrtl ModuleGraph_oriented.
+
+
+
+(*****************************************************************************)
+(*                                                                           *)
+(*                    P R E C O N D I T I O N   C H E C K S                  *)
+(*                                                                           *)
+(*****************************************************************************)
+
+
+
+(* The following functions allow to verify some preconditions for
+   Expand Whens.  In particular,
+   - whether everything has been fully inferred
+   - type checking functions *)
+
+(*---------------------------------------------------------------------------*)
+(* Ensuring that all types are fully inferred                                *)
+
+Definition fully_inferred (gt : fgtyp) : bool :=
+match gt with
+| Fuint_implicit _
+| Fsint_implicit _
+| Freset => false
+| _ => true
+end.
+
+Fixpoint ports_have_fully_inferred_ground_types (pp : seq HiFP.hfport) : bool :=
+match pp with
+| [::] => true
+| Finput  _ (Gtyp gt) :: pp'
+| Foutput _ (Gtyp gt) :: pp' => fully_inferred gt && ports_have_fully_inferred_ground_types pp'
+| _ => false
+end.
+
+Definition tmap_has_fully_inferred_ground_types (tmap : CEP.t (ftype * HiF.forient)) : Prop :=
+forall (v : ProdVarOrder.T),
+   match CEP.find v tmap return Prop with
+   | Some (Gtyp gt, _) => fully_inferred gt
+   | Some _ => False
+   | None => True
+   end.
+
+(*---------------------------------------------------------------------------*)
+(* Type checking references and expressions                                  *)
+
+Definition lhs_type_of_ref
+    (* finds the type of a ground-type reference that can be written
+       (i.e. no input ports and no nodes) *)
+    (ref : HiFP.href)         (* reference that is being written *)
+    (vm  : CEP.t vertex_type) (* part of the module graph that is in scope *)
+:   option fgtyp
+:=  match ref with
+    | Eid v =>
+        match CEP.find v vm with
+        | Some (OutPort gt)
+        | Some (Register gt _ _ _)
+        | Some (Wire gt) => Some gt
+        | _ => None
+        end
+    | _ => None (* TBD for memory and instances *)
+    end.
+
+Definition rhs_type_of_ref
+    (* finds the type of a ground-type reference that can be read
+       (i.e. no output ports) *)
+    (ref : HiFP.href)         (* reference that is being read *)
+    (vm  : CEP.t vertex_type) (* part of the module graph that is in scope *)
+:   option fgtyp
+:=  match ref with
+    | Eid v =>
+        match CEP.find v vm with
+        | Some (InPort gt)
+        | Some (Register gt _ _ _)
+        | Some (Wire gt)
+        | Some (Node gt) => Some gt
+        | _ => None
+        end
+    | _ => None (* TBD for memory and instances *)
+    end.
+
+Definition fgtyp_mux
+    (* Find the type of a multiplexer whose two inputs have types x and y, for ground types *)
+    (x y : fgtyp_explicit) (* the two inputs of the multiplexer *)
+:   option fgtyp_explicit
+:=  match x, y with
+    | exist (Fuint wx) _, exist (Fuint wy) _ => Some (Fuint_exp (maxn wx wy))
+    | exist (Fsint wx) _, exist (Fsint wy) _ => Some (Fsint_exp (maxn wx wy))
+    | exist Fclock _, exist Fclock _ => Some Fclock_exp
+    | exist Fasyncreset _, exist Fasyncreset _ => Some Fasyncreset_exp
+    | _, _ => None
+    end.
+
+Fixpoint rhs_type_of_expr 
+    (* Find the type of expression expr. It must be of a ground type. *)
+    (expr : HiFP.hfexpr)     (* expression whose type is constructed *)
+    (vm : CEP.t vertex_type) (* part of the module graph that is in scope *)
+:   option fgtyp_explicit
+:=  match expr with
+    | Econst t bs =>
+        match t with
+        | Fuint_implicit w => Some (Fuint_exp w)
+        | Fsint_implicit w => Some (Fsint_exp w)
+        | t => Some (exist not_implicit_width t I)
+        end
+    | Eref r =>
+        match rhs_type_of_ref r vm with
+        | Some (Fuint_implicit w) => Some (Fuint_exp w)
+        | Some (Fsint_implicit w) => Some (Fsint_exp w)
+        | Some t => Some (exist not_implicit_width t I)
+        | _ => None
+        end
+    | Ecast AsUInt e1 =>
+        match rhs_type_of_expr e1 vm with
+        | Some (exist (Fsint w) _)
+        | Some (exist (Fuint w) _) => Some (Fuint_exp w)
+        | Some (exist Fclock _)
+        | Some (exist Fasyncreset _) => Some (Fuint_exp 1)
+        | _ => None
+        end
+    | Ecast AsSInt e1 =>
+        match rhs_type_of_expr e1 vm with
+        | Some (exist (Fsint w) _)
+        | Some (exist (Fuint w) _) => Some (Fsint_exp w)
+        | Some (exist Fclock _)
+        | Some (exist Fasyncreset _) => Some (Fsint_exp 1)
+        | _ => None
+        end
+    | Ecast AsClock e1 =>
+        match rhs_type_of_expr e1 vm with
+        | Some _ => Some Fclock_exp
+        | _ => None
+        end
+    | Ecast AsAsync e1 =>
+        match rhs_type_of_expr e1 vm with
+        | Some _ => Some Fasyncreset_exp
+        | _ => None
+        end
+    | Eprim_unop (Upad n) e1 =>
+        match rhs_type_of_expr e1 vm with
+        | Some (exist (Fsint w) _) => Some (Fsint_exp (maxn w n))
+        | Some (exist (Fuint w) _) => Some (Fuint_exp (maxn w n))
+        | _ => None
+        end
+    | Eprim_unop (Ushl n) e1 =>
+        match rhs_type_of_expr e1 vm with
+        | Some (exist (Fsint w) _) => Some (Fsint_exp (w + n))
+        | Some (exist (Fuint w) _) => Some (Fuint_exp (w + n))
+        | _ => None
+        end
+    | Eprim_unop (Ushr n) e1 =>
+        match rhs_type_of_expr e1 vm with
+        | Some (exist (Fsint w) _) => Some (Fsint_exp (maxn (w - n) 1))
+        | Some (exist (Fuint w) _) => Some (Fuint_exp (maxn (w - n) 0))
+        | _ => None
+        end
+    | Eprim_unop Ucvt e1 =>
+        match rhs_type_of_expr e1 vm with
+        | Some (exist (Fsint w) _) => Some (Fsint_exp w)
+        | Some (exist (Fuint w) _) => Some (Fsint_exp (w + 1))
+        | _ => None
+        end
+    | Eprim_unop Uneg e1 =>
+        match rhs_type_of_expr e1 vm with
+        | Some (exist (Fsint w) _)
+        | Some (exist (Fuint w) _) => Some (Fsint_exp (w + 1))
+        | _ => None
+        end
+    | Eprim_unop Unot e1 =>
+        match rhs_type_of_expr e1 vm with
+        | Some (exist (Fsint w) _)
+        | Some (exist (Fuint w) _) => Some (Fuint_exp w)
+        | _ => None
+        end
+    | Eprim_unop (Uextr n1 n2) e1 =>
+        match rhs_type_of_expr e1 vm with
+        | Some (exist (Fsint w) _)
+        | Some (exist (Fuint w) _) =>
+            if (n2 <= n1) && (n1 < w) then Some (Fuint_exp (n1 - n2 + 1))
+                                      else None
+        | _ => None
+        end
+    | Eprim_unop (Uhead n) e1 =>
+        match rhs_type_of_expr e1 vm with
+        | Some (exist (Fsint w) _)
+        | Some (exist (Fuint w) _) =>
+            if n <= w then Some (Fuint_exp n)
+                      else None
+        | _ => None
+        end
+    | Eprim_unop (Utail n) e1 =>
+        match rhs_type_of_expr e1 vm with
+        | Some (exist (Fsint w) _)
+        | Some (exist (Fuint w) _) =>
+            if n <= w then Some (Fuint_exp (w - n))
+                      else None
+        | _ => None
+        end
+    | Eprim_unop _ e1 =>
+        match rhs_type_of_expr e1 vm with
+        | Some (exist (Fsint _) _)
+        | Some (exist (Fuint _) _) => Some (Fuint_exp 1)
+        | _ => None
+        end
+    | Eprim_binop (Bcomp _) e1 e2 =>
+        match rhs_type_of_expr e1 vm, rhs_type_of_expr e2 vm with
+        | Some (exist (Fsint _) _), Some (exist (Fsint _) _)
+        | Some (exist (Fuint _) _), Some (exist (Fuint _) _) => Some (Fuint_exp 1)
+        | _, _ => None
+        end
+    | Eprim_binop Badd e1 e2
+    | Eprim_binop Bsub e1 e2 =>
+        match rhs_type_of_expr e1 vm, rhs_type_of_expr e2 vm with
+        | Some (exist (Fuint w1) _), Some (exist (Fuint w2) _) => Some (Fuint_exp (maxn w1 w2 + 1))
+        | Some (exist (Fsint w1) _), Some (exist (Fsint w2) _) => Some (Fsint_exp (maxn w1 w2 + 1))
+        | _, _ => None
+        end
+    | Eprim_binop Bmul e1 e2 =>
+        match rhs_type_of_expr e1 vm, rhs_type_of_expr e2 vm with
+        | Some (exist (Fuint w1) _), Some (exist (Fuint w2) _) => Some (Fuint_exp (w1 + w2))
+        | Some (exist (Fsint w1) _), Some (exist (Fsint w2) _) => Some (Fsint_exp (w1 + w2))
+        | _, _ => None
+        end
+    | Eprim_binop Bdiv e1 e2 =>
+        match rhs_type_of_expr e1 vm, rhs_type_of_expr e2 vm with
+        | Some (exist (Fuint w1) _), Some (exist (Fuint w2) _) => Some (Fuint_exp w1)
+        | Some (exist (Fsint w1) _), Some (exist (Fsint w2) _) => Some (Fsint_exp (w1 + 1))
+        | _, _ => None
+        end
+    | Eprim_binop Brem e1 e2 =>
+        match rhs_type_of_expr e1 vm, rhs_type_of_expr e2 vm with
+        | Some (exist (Fuint w1) _), Some (exist (Fuint w2) _) => Some (Fuint_exp (minn w1 w2))
+        | Some (exist (Fsint w1) _), Some (exist (Fsint w2) _) => Some (Fsint_exp (minn w1 w2))
+        | _, _ => None
+        end
+    | Eprim_binop Bdshl e1 e2 =>
+        match rhs_type_of_expr e1 vm, rhs_type_of_expr e2 vm with
+        | Some (exist (Fuint w1) _), Some (exist (Fuint w2) _) => Some (Fuint_exp (2 ^ w2 + w1 - 1))
+        | Some (exist (Fsint w1) _), Some (exist (Fuint w2) _) => Some (Fsint_exp (2 ^ w2 + w1 - 1))
+        | _, _ => None
+        end
+    | Eprim_binop Bdshr e1 e2 =>
+        match rhs_type_of_expr e1 vm, rhs_type_of_expr e2 vm with
+        | Some (exist (Fuint w1) _), Some (exist (Fuint w2) _) => Some (Fuint_exp w1)
+        | Some (exist (Fsint w1) _), Some (exist (Fuint w2) _) => Some (Fsint_exp w1)
+        | _, _ => None
+        end
+    | Eprim_binop Bcat e1 e2 =>
+        match rhs_type_of_expr e1 vm, rhs_type_of_expr e2 vm with
+        | Some (exist (Fuint w1) _), Some (exist (Fuint w2) _)
+        | Some (exist (Fsint w1) _), Some (exist (Fsint w2) _) => Some (Fuint_exp (w1 + w2))
+        | _, _ => None
+        end
+    | Eprim_binop Band e1 e2
+    | Eprim_binop Bor e1 e2
+    | Eprim_binop Bxor e1 e2 =>
+        match rhs_type_of_expr e1 vm, rhs_type_of_expr e2 vm with
+        | Some (exist (Fuint w1) _), Some (exist (Fuint w2) _)
+        | Some (exist (Fsint w1) _), Some (exist (Fsint w2) _) => Some (Fuint_exp (maxn w1 w2))
+        | _, _ => None
+        end
+    | Emux c e1 e2 =>
+        match rhs_type_of_expr c vm, rhs_type_of_expr e1 vm, rhs_type_of_expr e2 vm with
+        | Some (exist (Fuint 1) _), Some t1, Some t2 => fgtyp_mux t1 t2
+        | _, _, _ => None
+        end
+    | Evalidif c e1 =>
+        match rhs_type_of_expr c vm with
+        | Some (exist (Fuint 1) _) => rhs_type_of_expr e1 vm
+        | _ => None
+        end
+    end.
+
+
+
+(*****************************************************************************)
+(*                                                                           *)
+(*                          M A I N   F U N C T I O N                        *)
+(*                                                                           *)
+(*****************************************************************************)
+
+
+
+Definition combine_when_connections
+    (* a helper function that takes two connection maps, generated
+       by the two branches of a when statement, and combines them
+       into one connection map containing suitable multiplexers *)
+    (cond           : HiFP.hfexpr)    (* condition under which to decide whether to take the value from true_conn_map *)
+    (true_conn_map  : CEP.t def_expr) (* connections made before or in the true branch *)
+    (false_conn_map : CEP.t def_expr) (* connections made before or in the false branch *)
+:   CEP.t def_expr
+:=  CEP.map2 (fun true_expr false_expr : option def_expr =>
+                      match true_expr, false_expr with
+                      | Some (D_fexpr te), Some (D_fexpr fe) =>
+                          if te == fe then true_expr
+                          else Some (D_fexpr (Emux cond te fe))
+                      | Some D_undefined, _
+                      | _, Some D_undefined => Some D_undefined
+                      | None, _ => false_expr
+                      | _, None => true_expr
+                      | Some D_invalidated, _ => false_expr
+                      | _, Some D_invalidated => true_expr
+                      end)
+             true_conn_map false_conn_map.
+
+Fixpoint ExpandBranches_funs
+    (* split a statement sequence (possibly containing when
+       statements) into a sequence that defines components and a
+       connection map.  The output does not contain when statements. *)
+    (ss           : HiFP.hfstmt_seq)   (* sequence of statements being translated *)
+    (old_comp_ss  : HiFP.hfstmt_seq)   (* component statements of earlier statements in the sequence (used for recursion) *)
+    (old_conn_map : CEP.t def_expr)    (* connections made by earlier statements in the sequence (used for recursion) *)
+    (old_scope    : CEP.t vertex_type) (* part of module graph vertices that is currently in scope *)
+:   option (HiFP.hfstmt_seq * CEP.t def_expr * CEP.t vertex_type)
+    (* old_comp_ss, extended with the component statements in ss,
+       old_conn_map, extended with the connection statements in ss,
+       and old_scope, extended with the component statements in ss that remain in scope *)
+:=  match ss with
+    | Qnil => Some (old_comp_ss, old_conn_map, old_scope)
+    | Qcons s ss =>
+        match ExpandBranch_fun s old_comp_ss old_conn_map old_scope with
+        | Some (temp_comp_ss, temp_conn_map, temp_scope) =>
+            ExpandBranches_funs ss temp_comp_ss temp_conn_map temp_scope
+        | None => None
+        end
+    end
+with ExpandBranch_fun
+    (* split a single statement (possibly consisting of a when
+       statement) into a sequence that defines components and a
+       connection map.  The output does not contain when statements. *)
+    (s            : HiFP.hfstmt)       (* a single statement being translated *)
+    (old_comp_ss  : HiFP.hfstmt_seq)   (* component statements of earlier statements in the sequence (used for recursion) *)
+    (old_conn_map : CEP.t def_expr)    (* connections made by earlier statements in the sequence (used for recursion) *)
+    (old_scope    : CEP.t vertex_type) (* part of module graph vertices that is currently in scope *)
+:   option (HiFP.hfstmt_seq * CEP.t def_expr * CEP.t vertex_type)
+    (* old_comp_ss, extended with the component statements in s,
+       old_conn_map, extended with the connection statements in s,
+       and old_scope, extended with the component statements in s that remain in scope *)
+:=  match s with
+    | Sskip => Some (old_comp_ss, old_conn_map, old_scope)
+    | Swire var (Gtyp typ) =>
+        (* no need to check whether var has been defined already.
+           It might still be handy though... we’ll see later. *)
+        Some (Qrcons old_comp_ss s, old_conn_map, CEP.add var (Wire typ) old_scope)
+    | Sreg var reg =>
+        (* we need to check whether the register definition contains
+           any expression with scoping errors *)
+        match type reg, rhs_type_of_expr (clock reg) old_scope, reset reg with
+        | Gtyp gt, Some _, Rst rst_sig rst_val =>
+            match rhs_type_of_expr rst_sig old_scope, rhs_type_of_expr rst_val old_scope with
+            | Some (exist Fasyncreset _), Some _ => Some (Qrcons old_comp_ss s, old_conn_map, CEP.add var (Register gt (clock reg) (reset reg) true) old_scope)
+            | Some (exist (Fuint 1) _), Some _ => Some (Qrcons old_comp_ss s, old_conn_map, CEP.add var (Register gt (clock reg) (reset reg) false) old_scope)
+            | _, _ => None
+            end
+        | Gtyp gt, Some _, NRst =>
+            Some (Qrcons old_comp_ss s, old_conn_map, CEP.add var (Register gt (clock reg) (reset reg) false) old_scope)
+        | _, _, _ => None
+        end
+    | Smem var mem => None
+    | Sinst var1 var2 => None
+    | Snode var expr =>
+        (* check whether the expression is in scope *)
+        match rhs_type_of_expr expr old_scope with
+        | Some (exist gt _) =>
+            Some (Qrcons old_comp_ss s, old_conn_map, CEP.add var (Node gt) old_scope)
+        | _ => None
+        end
+    | Sfcnct (Eid var) expr =>
+        (* The following code needs to be moved to a helper function
+           because ref can be more complex than just (Eid var). *)
+        (* check whether the two sides are in scope, and their flow direction is correct *)
+        match lhs_type_of_ref (Eid var) old_scope, rhs_type_of_expr expr old_scope with
+        | Some gt_tgt, Some (exist gt_src _) =>
+            if connect_type_compatible false (Gtyp gt_tgt) (Gtyp gt_src) false
+            then Some (old_comp_ss, CEP.add var (D_fexpr expr) old_conn_map, old_scope)
+            else None
+        | _, _ => None
+        end
+    | Sinvalid (Eid var) =>
+        match lhs_type_of_ref (Eid var) old_scope with
+        | Some _ =>
+            Some (old_comp_ss, CEP.add var D_invalidated old_conn_map, old_scope)
+        | _ => None
+        end
+    | Swhen cond ss_true ss_false =>
+        match rhs_type_of_expr cond old_scope with
+        | Some (exist (Fuint 1) _) =>
+            match ExpandBranches_funs ss_true old_comp_ss old_conn_map old_scope with
+            | Some (true_comp_ss, true_conn_map, _) =>
+                match ExpandBranches_funs ss_false true_comp_ss old_conn_map old_scope with
+                | Some (false_comp_ss, false_conn_map, _) =>
+                    Some (false_comp_ss, combine_when_connections cond true_conn_map false_conn_map, old_scope)
+                | _ => None
+                end
+            | _ => None
+            end
+        | _ => None
+        end
+    | _ => None
+    end.
+
+Fixpoint ExpandPorts_fun
+    (* create a map of def_expr for the port sequence pp.
+       Out ports need to be assigned value “undefined”;
+       in ports do not need to be assigned any value.
+       Because types have been lowered already, we can assume
+       that all ports have ground types. *)
+    (pp : seq HiFP.hfport) (* the sequence of ports of the module *)
+:   option (CEP.t vertex_type * CEP.t def_expr)
+:=  match pp with
+    | [::] => Some (CEP.empty vertex_type, CEP.empty def_expr)
+    | Finput p (Gtyp gt) :: pp' =>
+        match ExpandPorts_fun pp' with
+        | Some (vm_temp, ct_temp) =>
+            Some (CEP.add p (InPort gt) vm_temp, ct_temp)
+        | None => None
+        end
+    | Foutput p (Gtyp gt) :: pp' =>
+        match ExpandPorts_fun pp' with
+        | Some (vm_temp, ct_temp) =>
+            Some (CEP.add p (OutPort gt) vm_temp, CEP.add p D_undefined ct_temp)
+        | None => None
+        end
+    | _ => None
+    end.
+
+Definition convert_to_connect_stmts
+    (* converts a map of connections to connect statements *)
+    (conn_map : CEP.t def_expr) (* map that needs to be converted *)
+:   HiFP.hfstmt_seq
+:=  CEP.fold (fun (v : ProdVarOrder.t) (d : def_expr) (old_ss : HiFP.hfstmt_seq) =>
+                      match d with
+                      | D_undefined => old_ss
+                      | D_invalidated => Qcons (Sinvalid (Eid v)) old_ss
+                      | D_fexpr e => Qcons (Sfcnct (Eid v) e) old_ss
+                      end)
+             conn_map (Qnil ProdVarOrder.T).
+
+Definition ExpandWhens_fun
+    (* Expand When statements in a module *)
+    (m : HiFP.hfmodule) (* module that needs to be handled *)
+:   option HiFP.hfmodule (* result is either a semantically equivalent module without when statements,
+                            or nothing if there was some error *)
+:=  match m with
+    | FInmod v pp ss =>
+        match ExpandPorts_fun pp with
+        | Some (vm_port, ct_port) =>
+            match ExpandBranches_funs ss (Qnil ProdVarOrder.T) ct_port vm_port with
+            | Some (def_ss, conn_map, _) =>
+                Some (FInmod v pp (Qcat def_ss (convert_to_connect_stmts conn_map)))
+            | None => None
+            end
+        | None => None
+        end
+    | FExmod _ _ _ => None
+    end.
+
+
+
+(*****************************************************************************)
+(*                                                                           *)
+(*                      C O R R E C T N E S S   P R O O F                    *)
+(*                                                                           *)
+(*****************************************************************************)
+
+Lemma fully_inferred_does_not_change :
+forall (gt : fgtyp) (v : CEP.key) (vm : CEP.t vertex_type),
+   fully_inferred gt ->
+      match code_type_find_vm_widths (Gtyp gt) v vm with
+      | Some (Gtyp gt', _) => gt = gt'
+      | Some _ => False
+      | None => True
+      end.
+Proof.
+intros.
+unfold fully_inferred in H.
+destruct gt ; try discriminate H ; simpl code_type_find_vm_widths.
+* destruct (CEP.find v vm) as [[newgt|newgt|newgt _ _ _|newgt|newgt]|] ; try trivial ;
+  destruct newgt ; try trivial ; destruct (n == n0) eqn :Hnn0 ; try trivial ;
+  move /eqP : Hnn0 => Hnn0 ; rewrite -Hnn0 ; reflexivity.
+* destruct (CEP.find v vm) as [[newgt|newgt|newgt _ _ _|newgt|newgt]|] ; try trivial ;
+  destruct newgt ; try trivial ; destruct (n == n0) eqn :Hnn0 ; try trivial ;
+  move /eqP : Hnn0 => Hnn0 ; rewrite -Hnn0 ; reflexivity.
+* destruct (CEP.find v vm) as [[newgt|newgt|newgt _ _ _|newgt|newgt]|] ; try trivial ;
+  destruct newgt ; trivial.
+* destruct (CEP.find v vm) as [[newgt|newgt|newgt _ _ _|newgt|newgt]|] ; try trivial ;
+  destruct newgt ; trivial.
+Qed.
+
+Lemma ExpandPorts_fun_submap :
+    forall (ports : seq HiFP.hfport) (vm_old vm_new vm_port vm_old_port : CEP.t vertex_type)
+           (ct_old ct_new ct_port : CEP.t def_expr) (tmap port_tmap : CEP.t (ftype * HiF.forient)),
+    ports_have_fully_inferred_ground_types ports ->
+    ports_tmap ports vm_old_port = Some port_tmap ->
+    CEP.submap port_tmap tmap ->
+    ExpandPorts_fun ports = Some (vm_port, ct_port) ->
+        Sem_frag_ports vm_old ct_old ports vm_new ct_new tmap ->
+            CEP.submap vm_port vm_new.
+Proof.
+induction ports as [|port ports'] ; simpl ; intros.
+* injection H2 ; clear H2 ; intros ; subst vm_port ct_port.
+  intro.
+  by rewrite CEP.Lemmas.F.empty_o //.
+* intro.
+  (*generalize (ports_tmap_uniq vm_old_port (port :: ports')) ; intro.
+  simpl in H4.
+  rewrite H0 in H4.*)
+  destruct port as [port_name [port_fgtyp| |]|port_name [port_fgtyp| |]] ;
+        try by discriminate H2.
+  1-2: destruct (ExpandPorts_fun ports') as [[vm_temp ct_temp]|] ;
+        last by discriminate H2.
+  1-2: injection H2 ; clear H2 ; intros ; subst vm_port ct_port.
+  1-2: destruct H3 as [vm' [ct' H3]].
+  1-2: move /andP : H => H.
+  1-2: specialize (IHports' vm_old vm' vm_temp vm_old_port ct_old ct' ct_temp tmap)
+                  with (1 := proj2 H) (4 := Logic.eq_refl).
+  1-2: generalize (fully_inferred_does_not_change port_fgtyp port_name vm_old_port (proj1 H)) ; intro.
+  1-2: destruct (code_type_find_vm_widths (Gtyp port_fgtyp) port_name vm_old_port)
+       as [[[port_fgtyp'| |] _]|] ;
+             last (by discriminate H0) ;
+             try (by contradiction H2) ;
+             subst port_fgtyp'.
+  1-2: destruct (ports_tmap ports' vm_old_port) as [temp_tmap|] ;
+             last by discriminate H0.
+  1-2: specialize (IHports' temp_tmap Logic.eq_refl) with (2 := proj1 H3).
+  1-2: destruct H3 as [_ H3] ; simpl Sem_frag_port in H3.
+  1-2: destruct (CEP.find port_name temp_tmap) eqn: H2 ; first by discriminate H0.
+  1-2: injection H0 ; clear H0 ; intros ; subst port_tmap.
+  1-2: rewrite (CEP.Lemmas.submap_add_find H1) in H3.
+  1-2: specialize (IHports' (CEP.Lemmas.submap_add_find_none H1 H2)).
+  1-2: destruct (k == port_name) eqn: Hport_name_k.
+  - 1,3: rewrite CEP.Lemmas.find_add_eq // in H5.
+    1-2: move /eqP : Hport_name_k => Hport_name_k ; subst k.
+    1-2: injection H5 ; clear H5 ; intros ; subst v.
+    1-2: destruct H3 as [H3 _] ; simpl connect_port in H3.
+    1-2: move /and3P : H3 => [/andP [_ /eqP H3] _ _].
+    1-2: exact H3.
+  - 1-2: destruct H3 as [_ H3].
+    1-2: specialize (H3 k.1 k.2).
+    1-2: rewrite /size_of_ftype -surjective_pairing add1n in H3.
+    1-2: assert (k.1 <> port_name.1 \/ k.2 < port_name.2 \/ port_name.2 < k.2).
+          1,3: clear -Hport_name_k.
+          1-2: destruct (k.1 != port_name.1) eqn: H1 ;
+                     first (by left ; move /eqP : H1 => H1 ; exact H1).
+          1-2: destruct (k.2 < port_name.2) eqn: H2small ;
+                     first (by right ; left ; reflexivity).
+          1-2: destruct (port_name.2 < k.2) eqn: H2large ;
+                     first (by right ; right ; reflexivity).
+          1-2: move /eqP : H1 => H1.
+          1-2: apply injective_projections in H1 ;
+                     first by rewrite H1 eq_refl // in Hport_name_k.
+          1-2: assert (nat_of_bin k.2 == nat_of_bin port_name.2)
+                     by rewrite eqn_leq leqNgt H2large leqNgt H2small //.
+Admitted.
+
+Lemma ports_tmap_and_ExpandPorts_fun :
+    (* a lemma that relates ports_tmap and ExpandPorts_fun *)
+    forall (ports : seq HiFP.hfport) (vm_port vm : CEP.t vertex_type) (ct_port : CEP.t def_expr) (pmap : CEP.t (ftype * HiF.forient)),
+    ports_have_fully_inferred_ground_types ports ->
+    ExpandPorts_fun ports = Some (vm_port, ct_port) ->
+    ports_tmap ports vm = Some pmap ->
+            (forall v : CEP.key,
+                match CEP.find v pmap with
+                | Some (Atyp _ _, _) | Some (Btyp _, _) => False
+                | _ => True
+                end)
+        /\
+            CEP.Equal vm_port (CEP.map (fun el : ftype * HiF.forient =>
+                                               match el with
+                                               | (Gtyp gt, HiF.Source) => InPort gt
+                                               | (Gtyp gt, HiF.Sink) => OutPort gt
+                                               | _ => Node Freset
+                                               end)
+                                       pmap)
+        /\
+            CEP.Equal ct_port (CEP.map2 (fun (el : option (ftype * HiF.forient)) (_ : option unit) =>
+                                               match el with
+                                               | Some (Gtyp gt, HiF.Sink) => Some D_invalidated
+                                               | _ => None
+                                               end)
+                                       pmap (CEP.empty unit)).
+Proof.
+induction ports as [|port ports'] ; simpl ; intros.
+* injection H0 ; clear H H0 ; intros ; subst vm_port ct_port.
+  injection H1 ; clear H1 ; intros ; subst pmap.
+  split.
+  + intro.
+    by rewrite CEP.Lemmas.F.empty_o //.
+  split.
+  + intro.
+    rewrite CEP.Lemmas.F.empty_o.
+    symmetry ; apply CEP.Lemmas.F.not_find_in_iff ; intro.
+    apply CEP.map_2, CEP.Lemmas.empty_in_iff in H.
+    exact H.
+  + intro.
+    by rewrite CEP.Lemmas.F.empty_o CEP.Lemmas.F.map2_1bis //.
+* split.
+  + intro.
+    destruct port as [port_name [port_fgtyp| |]|port_name [port_fgtyp| |]] ;
+          try by discriminate H0.
+    1,2: destruct (v == port_name) eqn: Hport_name_v.
+    - 1,3: move /eqP : Hport_name_v => Hport_name_v.
+      1-2: subst v.
+      1-2: simpl code_type_find_vm_widths in H1.
+      1-2: destruct (CEP.find port_name vm) as [[newgt|newgt|newgt _ _ _|newgt|newgt]|] ; last (by discriminate H1).
+        1-10: destruct (code_vm_type_equivalent port_fgtyp newgt) ; last (by discriminate H1).
+        1-10: destruct (ports_tmap ports' vm) ; last by discriminate H1.
+        1-10: destruct (CEP.find port_name t) ; first by discriminate H1.
+        1-10: injection H1 ; clear H1 ; intros ; subst pmap.
+        1-10: rewrite CEP.Lemmas.find_add_eq // /PVM.SE.eq //.
+    - 1-2: destruct (code_type_find_vm_widths (Gtyp port_fgtyp) port_name vm) as [[newt _]|] ; last by discriminate H1.
+      1-2: move /andP : H => [_ H].
+      1-2: destruct (ExpandPorts_fun ports') as [[vm_temp ct_temp]|] ; last by discriminate H0.
+      1-2: specialize (IHports' vm_temp vm ct_temp) with (1 := H) (2 := Logic.eq_refl).
+      1-2: destruct (ports_tmap ports' vm) as [pmap'|] ; last by discriminate H1.
+      1-2: specialize (IHports' pmap' Logic.eq_refl).
+      1-2: destruct IHports' as [IHports' _].
+      1-2: specialize (IHports' v).
+      1-2: destruct (CEP.find port_name pmap') ; first by discriminate H1.
+      1-2: injection H1 ; clear H1 ; intros ; subst pmap.
+      1-2: by rewrite CEP.Lemmas.find_add_neq // /PVM.SE.eq Hport_name_v //.
+  split.
+  + intro.
+    rewrite CEP.Lemmas.map_o.
+    destruct port as [port_name [port_fgtyp| |]|port_name [port_fgtyp| |]] ;
+          try by discriminate H0.
+    1,2: destruct (y == port_name) eqn: Hport_name_y.
+    - 1,3: move /eqP : Hport_name_y => Hport_name_y.
+      1-2: subst y.
+      1-2: generalize (ExpandPorts_fun_submap ports') ; intro.
+      1-2: destruct (ExpandPorts_fun ports') as [[vm_temp ct_temp]|] ; last by discriminate H0.
+      1-2: injection H0 ; clear H0 ; intros ; subst vm_port ct_port.
+      1-2: rewrite CEP.Lemmas.find_add_eq // ; last by rewrite /PVM.SE.eq //.
+      1-2: simpl code_type_find_vm_widths in H1.
+      1-2: destruct (CEP.find port_name vm) as [[newgt|newgt|newgt _ _ _|newgt|newgt]|] ; last (by discriminate H1).
+        1-10: destruct (code_vm_type_equivalent port_fgtyp newgt) ; last (by discriminate H1).
+        1-10: destruct (ports_tmap ports' vm) ; last by discriminate H1.
+        1-10: destruct (CEP.find port_name t) ; first by discriminate H1.
+        1-10: injection H1 ; clear H1 ; intros ; subst pmap.
+        1-10: rewrite CEP.Lemmas.find_add_eq // /option_map /PVM.SE.eq //.
+    - 1-2: destruct (code_type_find_vm_widths (Gtyp port_fgtyp) port_name vm) as [[newt _]|] ; last by discriminate H1.
+      1-2: move /andP : H => [_ H].
+      1-2: destruct (ExpandPorts_fun ports') as [[vm_temp ct_temp]|] ; last by discriminate H0.
+      1-2: specialize (IHports' vm_temp vm ct_temp) with (1 := H) (2 := Logic.eq_refl).
+      1-2: destruct (ports_tmap ports' vm) as [pmap'|] ; last by discriminate H1.
+      1-2: specialize (IHports' pmap' Logic.eq_refl).
+      1-2: destruct IHports' as [IHports' _].
+      1-2: specialize (IHports' v).
+      1-2: destruct (CEP.find port_name pmap') ; first by discriminate H1.
+      1-2: injection H1 ; clear H1 ; intros ; subst pmap.
+      1-2: by rewrite CEP.Lemmas.find_add_neq // /PVM.SE.eq Hport_name_v //.
+    admit.
+  + admit.
+Admitted.
+
+Theorem ExpandWhens_correct :
+(* if ExpandWhens creates a new module and it has a certain semantic,
+   then the previous module also has the same semantic. *)
+    forall (m m' : HiFP.hfmodule)
+           (vm : CEP.t vertex_type) (ct : CEP.t def_expr),
+        ExpandWhens_fun m = Some m' ->
+        Sem m' vm ct ->
+            Sem m vm ct.
+Proof.
+intros.
+unfold ExpandWhens_fun in H.
+unfold Sem, ports_stmts_tmap in H0.
+unfold Sem, ports_stmts_tmap.
+destruct m as [m_name m_ports m_stmts|]; try by discriminate H.
+destruct (ExpandPorts_fun) as [[vm_port ct_port]|] eqn: HExpandPorts ; try by discriminate H.
+destruct (ExpandBranches_funs m_stmts (Qnil ProdVarOrder.T) ct_port vm_port)
+         as [[[def_ss conn_map] final_scope]|] eqn: HexpandBranches ; try by discriminate H.
+injection H ; clear H ; intros ; subst m'.
+destruct (ports_tmap m_ports vm) as [pmap|] ; try by contradiction H0.
+generalize (stmts_tmap_components vm m_stmts pmap pmap pmap
+            (CEP.Lemmas.submap_refl pmap) (CEP.Lemmas.submap_refl pmap) (CEP.Lemmas.submap_refl pmap)) ; intro.
+(* use a lemma to ensure that 
+stmts_tmap (pmap, pmap) (Qcat def_ss ...) vm =
+stmts_tmap (pmap, pmap) m_stmts           vm.
+*)
+
+
+
+
+
+
+
+
+
+
+
+
+
+
+
+
+
+
+
+
+
+
+
+
+ExpandPorts_fun m_ports = Some (vm_port, ct_port) ->
+    ports_tmap m_ports vm = Some pmap ->
+            (forall v : CEP.key,
+                match CEP.find v pmap with
+                | Some (Atyp _ _, _) | Some (Btyp _, _) => False
+                | _ => True
+                end)
+        /\
+            CEP.Equal vm_port (CEP.map (fun el : ftype * HiF.forient =>
+                                               match el with
+                                               | (Gtyp gt, HiF.Source) => InPort gt
+                                               | (Gtyp gt, HiF.Sink) => OutPort gt
+                                               | _ => Node Freset)
+                                       pmap)
+        /\
+            CEP.Equal ct_port (CEP.map2 (fun el _ : option (ftype * HiF.forient) =>
+                                               match el with
+                                               | Some (Gtyp gt, HiF.Sink) => Some D_invalidated
+                                               | _ => None)
+                                       pmap)
+
+    (forall v1 v2 : N,
+     match CEP.find (v1, v2) tmap with
+     | Some (Atyp _ _, _) | Some (Btyp _, _) =>
+         forall v2' : N, v2' <> v2 -> CEP.find (v1, v2') tmap = None
+     | _ => True
+     end) /\
+
+
